initial tactics pass

Main.lean
@@ -1,24 +1,23 @@
 import Pauline.Notation
 import Pauline.Statics
+import Pauline.Tactic
+import Mathlib.Tactic
+import Mathlib.Data.String.Lemmas
 
-open Pauline
+open Pauline Pauline.Tactic
 
 def fact := [sml|
-
   fun fact (n : int) : int =
     if n = 0
     then 1
     else n * fact (n - 1)
-
 ]
 
 def program_ctx : Context := sorry
-def program_state : State :=
+abbrev program_state : State := -- todo automate
   let init : State := default
-  ⟨ Std.HashMap.insert init.values "fact" -- todo automate
-      ⟨[sml_exp| fn n => if n = 0 then 1 else n * fact (n - 1)], by decide⟩
-  ⟩
-#eval eval program_state [sml_exp| fact 12]
+  init.insert "fact"
+    ⟨[sml_exp| fn n => if n = 0 then 1 else n * fact (n - 1)], by decide⟩
 
 theorem fact_tc
   : [smlprop|
@@ -27,12 +26,32 @@ theorem fact_tc
   := by
   sorry
 
-elab "sml_eval" : tactic =>
-  Lean.Elab.Tactic.withMainContext do
-    let goal ← Lean.Elab.Tactic.getMainTarget
-    let expr_type ← Lean.Meta.inferType goal
-    dbg_trace f!"goal: {goal}"
+-- #eval step program_state [sml_exp| if 0 = 0 then 1 else n * fact (n - 1)]
 
+abbrev test := [sml_exp| if true then (if false then 0 else 1) else 2]
+
+example : [smlprop|
+           program_state ⊢ if 1 = 1 then (if false then 0 else 1) else 2
+      ==>* program_state ⊢ 1
+    ] := by
+  repeat sml_step
+
+example : [smlprop|
+           program_state ⊢ if 1 = 1 then 1 else 0
+      ==>* program_state ⊢ 1
+    ] := by
+  repeat sml_step
+
+example : [smlprop|
+           program_state ⊢ fact 0
+      ==>* program_state ⊢ 1
+    ] := by
+  sml_step
+  sml_step
+  sml_step
+  simp
+  -- sml_eval'
+  sorry
 
 theorem fact_requires_total
   : ∀ n : Nat, n ≥ 0 → ∃ v : Nat,
@@ -43,19 +62,39 @@ theorem fact_requires_total
   intro n requires
   induction n
   case zero =>
-    refine ⟨0, ?_⟩
-    sml_eval
+    refine ⟨1, ?_⟩
+    let fact0 := [sml_exp| fact ↑0]
+    let res := eval program_state fact0
+    -- sml_eval
     (calc
-      (program_state, [sml_exp| fact ↑0])
-      ==>* (program_state, [sml_exp| 0]) := by sorry
+             (program_state, [sml_exp| fact ↑0])
+        ==>* (program_state, [sml_exp| if ↑0 = 0 then 1 else n * fact (n - 1)])
+          := by sorry
+      _ ==>* (program_state, [sml_exp| if true then 1 else n * fact (n - 1)])
+          := by sorry
+      _ ==>* (program_state, [sml_exp| 1])
+          := by refine ⟨1, ?_⟩
+                exact .iteStepT rfl
+      _ ==>* (program_state, [sml_exp| 1])
+          := by try (refine ⟨0, ?_⟩; simp)
     )
   case succ n' ih =>
-    simp at *
-    have v' := ih.choose
-    refine ⟨n' * v', ?_⟩
+    simp at ih
+    let v' := ih.choose
+    have := ih.choose_spec
+    refine ⟨n' * ih.choose, ?_⟩
     (calc
              (program_state, [sml_exp| fact (↑(n' + 1))])
-        ==>* (program_state, [sml_exp| ↑n' * fact (↑n' - 1)]) := by sorry
-      _ ==>* (program_state, [sml_exp| ↑n' * ↑v'])            := by sorry -- ih
+        ==>* (program_state, [sml_exp| ↑n' * fact ↑n']) := by sorry
+      _ ==>* (program_state, [sml_exp| ↑n' * ↑v'])
+          := by apply StepsExp.trans
+                case y => exact (program_state, ih.choose)
+                apply Exists.intro 1
+                simp
+                sorry
+                -- exact .tupleTlStep sorry sorry
+                -- sorry
+                -- exact ih.choose_spec
+                sorry
       _ ==>* (program_state, [sml_exp| ↑(n' * v')])          := by sorry
     )
