Pauline/Tactic.lean
@@ -1,0 +1,97 @@
+import Std
+import Pauline.Dynamics
+
+namespace Pauline.Tactic
+
+/-
+open Lean Lean.Expr Lean.Meta
+
+elab "sml_eval'" : tactic =>
+  Lean.Elab.Tactic.withMainContext do
+    let goal ← Lean.Elab.Tactic.getMainTarget
+    let expr_type ← Lean.Meta.inferType goal
+    dbg_trace f!"goal: {goal}\n\n{expr_type}"
+
+def myApply (goal : MVarId) (e : Expr) : MetaM (List MVarId) := do
+  -- Check that the goal is not yet assigned.
+  goal.checkNotAssigned `myApply
+  -- Operate in the local context of the goal.
+  goal.withContext do
+    -- Get the goal's target type.
+    let target ← goal.getType
+    -- Get the type of the given expression.
+    let type ← inferType e
+    -- If `type` has the form `∀ (x₁ : T₁) ... (xₙ : Tₙ), U`, introduce new
+    -- metavariables for the `xᵢ` and obtain the conclusion `U`. (If `type` does
+    -- not have this form, `args` is empty and `conclusion = type`.)
+    let (args, _, conclusion) ← forallMetaTelescopeReducing type
+    -- If the conclusion unifies with the target:
+    if ← isDefEq target conclusion then
+      -- Assign the goal to `e x₁ ... xₙ`, where the `xᵢ` are the fresh
+      -- metavariables in `args`.
+      goal.assign (mkAppN e args)
+      -- `isDefEq` may have assigned some of the `args`. Report the rest as new
+      -- goals.
+      let newGoals ← args.filterMapM λ mvar => do
+        let mvarId := mvar.mvarId!
+        if ! (← mvarId.isAssigned) && ! (← mvarId.isDelayedAssigned) then
+          return some mvarId
+        else
+          return none
+      return newGoals.toList
+    -- If the conclusion does not unify with the target, throw an error.
+    else
+      throwTacticEx `myApply goal m!"{e} is not applicable to goal with target {target}"
+
+elab "sml_step'" : tactic =>
+  Lean.Elab.Tactic.withMainContext do
+    sorry
+-/
+
+macro "sml_step_rfl" : tactic =>
+  `(tactic| exact ⟨0, by simp⟩)
+
+macro "sml_step_extern" : tactic =>
+  `(tactic| ( apply StepExp.externStep
+              rfl
+              decide
+            )
+   )
+
+macro "sml_step_apply" : tactic =>
+  `(tactic| ( apply StepExp.appStep
+              rfl
+              decide
+            )
+   )
+
+macro "sml_step_one" : tactic =>
+  `(tactic| ( first | exact StepExp.tupleNilStep
+                    | sml_step_extern
+                    | sml_step_apply
+                    | exact StepExp.typedStep
+                    | apply StepExp.varStep (by constructor)
+                    | apply StepExp.appStepL (by decide)
+                    | apply StepExp.appStepR
+                    | apply StepExp.raiseStep
+                    | exact StepExp.iteStepT rfl
+                    | exact StepExp.iteStepF rfl
+                    | apply StepExp.iteStepB
+              --  (apply .tupleHdStep; sorry))
+            )
+   )
+
+macro "sml_step_star" : tactic =>
+  `(tactic| ( apply StepsExp.trans
+              apply Exists.intro 1
+              sml_step_one
+            )
+   )
+
+macro "sml_step" : tactic =>
+  `(tactic| first | sml_step_star
+                  | sml_step_one
+                  | sml_step_rfl
+   )
+
+-- todo make SML tactic specific syntax category
